Foundation.lean
@@ -182,7 +182,7 @@ import Foundation.ProvabilityLogic.Grz.Completeness
 import Foundation.ProvabilityLogic.S.Completeness
 
 import Foundation.ProvabilityLogic.Classification.LetterlessTrace
-import Foundation.ProvabilityLogic.Classification.GeneralizedTrace
+import Foundation.ProvabilityLogic.Classification.Trace
 
 import Foundation.Meta.Qq
 import Foundation.Meta.Lit
